Foundation.lean
@@ -118,6 +118,7 @@ import Foundation.Modal.Kripke.LinearFrame
 import Foundation.Modal.PLoN.Logic.N
 
 import Foundation.Modal.Neighborhood.Logic.EMCN
+import Foundation.Modal.Neighborhood.Logic.E4
 
 import Foundation.Modal.ModalCompanion.Int
 import Foundation.Modal.ModalCompanion.KC
