Foundation/Modal/Neighborhood/Logic/E4.lean
@@ -1,0 +1,69 @@
+import Foundation.Modal.Neighborhood.Hilbert
+import Foundation.Modal.Neighborhood.AxiomGeach
+import Foundation.Modal.Neighborhood.Logic.E
+
+namespace LO.Modal
+
+open Neighborhood
+open Hilbert.Neighborhood
+open Formula.Neighborhood
+
+namespace Neighborhood
+
+@[reducible] protected alias Frame.IsE4 := Frame.IsTransitive
+protected abbrev FrameClass.E4 : FrameClass := { F | F.IsE4 }
+
+end Neighborhood
+
+
+namespace Hilbert
+
+namespace E4.Neighborhood
+
+instance : Sound Hilbert.E4 FrameClass.E4 := instSound_of_validates_axioms $ by
+  simp only [Semantics.RealizeSet.singleton_iff];
+  intro F hF;
+  replace hF := Set.mem_setOf_eq.mp hF;
+  apply valid_axiomFour_of_isTransitive;
+
+instance : Entailment.Consistent Hilbert.E4 := consistent_of_sound_frameclass FrameClass.E4 $ by
+  use Frame.simple_blackhole;
+  simp only [Set.mem_setOf_eq];
+  constructor;
+  simp [Frame.box, Frame.box_iterate];
+
+end E4.Neighborhood
+
+instance : Hilbert.E ⪱ Hilbert.E4 := by
+  constructor;
+  . apply Hilbert.WithRE.weakerThan_of_subset_axioms;
+    simp;
+  . apply Entailment.not_weakerThan_iff.mpr;
+    use (Axioms.Four (.atom 0));
+    constructor;
+    . simp;
+    . apply Sound.not_provable_of_countermodel (𝓜 := FrameClass.E);
+      apply not_validOnFrameClass_of_exists_frame;
+      use {
+        World := Fin 2,
+        𝒩 w :=
+          match w with
+          | 0 => ∅
+          | 1 => {{0, 1}},
+      };
+      constructor;
+      . tauto;
+      . apply not_imp_not.mpr isTransitive_of_valid_axiomFour;
+        by_contra hC;
+        have := @(hC.trans {0, 1});
+        have := @this 1 ?_;
+        . have := Set.Subset.antisymm_iff.mp this |>.2;
+          have := @this 0;
+          simp at this;
+        . simp [Frame.box]
+
+end Hilbert
+
+instance : 𝐄 ⪱ 𝐄𝟒 := inferInstance
+
+end LO.Modal
