Foundation/Modal/Neighborhood/Logic/EMCN.lean
@@ -81,10 +81,7 @@ instance : Hilbert.ECN ⪱ Hilbert.EMCN := by
       apply not_validOnFrameClass_of_exists_model_world;
       let M : Model := {
         World := Fin 2,
-        𝒩 := λ w =>
-          match w with
-          | 0 => {∅, {0, 1}}
-          | 1 => {∅, {0, 1}},
+        𝒩 := λ w => {∅, {0, 1}},
         Val := λ w =>
           match w with
           | 0 => {0}
@@ -99,12 +96,10 @@ instance : Hilbert.ECN ⪱ Hilbert.EMCN := by
             match x with | 0 | 1 => simp_all [M, Set.Fin2.eq_univ];
           regular := by
             rintro X Y w ⟨hwX, hwY⟩;
-            match w with
-            | 0 | 1 =>
-              simp_all only [Fin.isValue, Set.mem_setOf_eq, Set.mem_insert_iff, Set.mem_singleton_iff, M];
-              rcases hwX with (rfl | rfl) <;>
-              rcases hwY with (rfl | rfl) <;>
-              simp;
+            simp_all only [Fin.isValue, Set.mem_setOf_eq, Set.mem_insert_iff, Set.mem_singleton_iff, M];
+            rcases hwX with (rfl | rfl) <;>
+            rcases hwY with (rfl | rfl) <;>
+            simp;
         }
       . simp! [M, Semantics.Realize, Satisfies];
         tauto_set;
